src/cbor/CBOR.Spec.Raw.Valid.fsti
@@ -82,7 +82,7 @@ let valid_raw_data_item
 : Tot bool
 = holds_on_raw_data_item valid_raw_data_item_elem l
 
-let rec raw_equiv_sorted_optimal
+val raw_equiv_sorted_optimal
   (order: raw_data_item -> raw_data_item -> bool {
     order_irrefl order /\
     order_trans order
@@ -97,153 +97,8 @@ let rec raw_equiv_sorted_optimal
     raw_data_item_ints_optimal x2
   ))
   (ensures (x1 == x2))
-  (decreases x1)
-= raw_equiv_eq x1 x2;
-  holds_on_raw_data_item_eq (raw_data_item_sorted_elem order) x1;
-  holds_on_raw_data_item_eq (raw_data_item_sorted_elem order) x2;
-  holds_on_raw_data_item_eq raw_data_item_ints_optimal_elem x1;
-  holds_on_raw_data_item_eq raw_data_item_ints_optimal_elem x2;
-  match x1, x2 with
-  | Simple _, Simple _ -> ()
-  | Int64 _ v1, Int64 _ v2 ->
-    raw_uint64_optimal_unique v1 v2
-  | String _ v1 _, String _ v2 _ ->
-    raw_uint64_optimal_unique v1 v2
-  | Tagged tag1 v1, Tagged tag2 v2 ->
-    raw_uint64_optimal_unique tag1 tag2;
-    raw_equiv_sorted_optimal order v1 v2
-  | Array len1 l1, Array len2 l2 ->
-    raw_uint64_optimal_unique len1 len2;
-    assert_norm (raw_data_item_ints_optimal == holds_on_raw_data_item raw_data_item_ints_optimal_elem);
-    list_for_all2_prod (raw_data_item_sorted order) (raw_data_item_sorted order) l1 l2;
-    list_for_all2_prod raw_data_item_ints_optimal raw_data_item_ints_optimal l1 l2;
-    list_for_all2_andp_intro
-      (prodp (raw_data_item_sorted order) (raw_data_item_sorted order))
-      (prodp raw_data_item_ints_optimal raw_data_item_ints_optimal)
-      l1 l2;
-    list_for_all2_andp_intro
-      (andp2
-        (prodp (raw_data_item_sorted order) (raw_data_item_sorted order))
-        (prodp raw_data_item_ints_optimal raw_data_item_ints_optimal))
-      raw_equiv
-      l1 l2;
-    list_for_all2_implies
-      (andp2
-        (andp2
-          (prodp (raw_data_item_sorted order) (raw_data_item_sorted order))
-          (prodp raw_data_item_ints_optimal raw_data_item_ints_optimal))
-        raw_equiv
-      )
-      ( = )
-      l1 l2
-      (fun x1' x2' ->
-        raw_equiv_sorted_optimal order x1' x2'
-      );
-    list_for_all2_equals l1 l2
-  | Map len1 l1, Map len2 l2 ->
-    raw_uint64_optimal_unique len1 len2;
-    assert_norm (raw_data_item_ints_optimal == holds_on_raw_data_item raw_data_item_ints_optimal_elem);
-    list_for_all_andp (holds_on_pair (raw_data_item_sorted order)) (holds_on_pair raw_data_item_ints_optimal) l1;
-    list_for_all_andp (holds_on_pair (raw_data_item_sorted order)) (holds_on_pair raw_data_item_ints_optimal) l2;
-    list_for_all_exists_prodp
-      (holds_on_pair2 raw_equiv)
-      (andp
-        (holds_on_pair (raw_data_item_sorted order))
-        (holds_on_pair raw_data_item_ints_optimal)
-      )
-      (andp
-        (holds_on_pair (raw_data_item_sorted order))
-        (holds_on_pair raw_data_item_ints_optimal)
-      )
-      l1 l2;
-    list_for_all_exists_implies
-      (andp2
-        (holds_on_pair2 raw_equiv)
-        (prodp
-          (andp
-            (holds_on_pair (raw_data_item_sorted order))
-            (holds_on_pair raw_data_item_ints_optimal)
-          )
-          (andp
-            (holds_on_pair (raw_data_item_sorted order))
-            (holds_on_pair raw_data_item_ints_optimal)
-          )
-        )
-      )
-      ( = )
-      l1 l2
-      (fun x1 x2 ->
-        raw_equiv_sorted_optimal order (fst x1) (fst x2);
-        raw_equiv_sorted_optimal order (snd x1) (snd x2)
-      );
-    list_for_all_exists_equal_eq l1 l2;
-    list_for_all_exists_prodp
-      (holds_on_pair2 raw_equiv)
-      (andp
-        (holds_on_pair (raw_data_item_sorted order))
-        (holds_on_pair raw_data_item_ints_optimal)
-      )
-      (andp
-        (holds_on_pair (raw_data_item_sorted order))
-        (holds_on_pair raw_data_item_ints_optimal)
-      )
-      l2 l1;
-    list_for_all_exists_implies
-      (andp2
-        (holds_on_pair2 raw_equiv)
-        (prodp
-          (andp
-            (holds_on_pair (raw_data_item_sorted order))
-            (holds_on_pair raw_data_item_ints_optimal)
-          )
-          (andp
-            (holds_on_pair (raw_data_item_sorted order))
-            (holds_on_pair raw_data_item_ints_optimal)
-          )
-        )
-      )
-      ( = )
-      l2 l1
-      (fun x2 x1 ->
-        raw_equiv_sym (fst x2) (fst x1);
-        raw_equiv_sorted_optimal order (fst x1) (fst x2);
-        raw_equiv_sym (snd x2) (snd x1);
-        raw_equiv_sorted_optimal order (snd x1) (snd x2)
-      );
-    list_for_all_exists_equal_eq l2 l1;
-    list_sorted_ext_eq (map_entry_order order _) l1 l2
 
-let rec raw_data_item_sorted_optimal_valid_aux
-  (order: (raw_data_item -> raw_data_item -> bool) {
-    order_irrefl order /\
-    order_trans order
-  })
-  (l: list (raw_data_item & raw_data_item))
-: Lemma
-  (requires (
-    List.Tot.for_all (holds_on_pair (raw_data_item_sorted order)) l /\
-    List.Tot.for_all (holds_on_pair raw_data_item_ints_optimal) l /\
-    FStar.List.Tot.sorted (map_entry_order order _) l
-  ))
-  (ensures (
-    list_no_setoid_repeats (map_entry_order raw_equiv _) l
-  ))
-  (decreases l)
-= match l with
-  | [] -> ()
-  | a :: q ->
-    raw_data_item_sorted_optimal_valid_aux order q;
-    if List.Tot.existsb (map_entry_order raw_equiv _ a) q
-    then begin
-      let a' = list_existsb_elim (map_entry_order raw_equiv _ a) q in
-      list_sorted_memP (map_entry_order order _) a q a';
-      List.Tot.for_all_mem (holds_on_pair (raw_data_item_sorted order)) q;
-      List.Tot.for_all_mem (holds_on_pair (raw_data_item_ints_optimal)) q;
-      raw_equiv_sorted_optimal order (fst a) (fst a')
-    end
-    else ()
-
-let raw_data_item_sorted_optimal_valid
+val raw_data_item_sorted_optimal_valid
   (order: raw_data_item -> raw_data_item -> bool {
     order_irrefl order /\
     order_trans order
@@ -255,20 +110,205 @@ let raw_data_item_sorted_optimal_valid
     raw_data_item_ints_optimal x1
   ))
   (ensures (valid_raw_data_item x1))
-= holds_on_raw_data_item_andp (raw_data_item_sorted_elem order) raw_data_item_ints_optimal_elem x1;
-  holds_on_raw_data_item_implies
-    (andp (raw_data_item_sorted_elem order) raw_data_item_ints_optimal_elem)
-    valid_raw_data_item_elem
-    (fun x ->
-      match x with
-      | Map len v ->
-        holds_on_raw_data_item_andp (raw_data_item_sorted_elem order) raw_data_item_ints_optimal_elem x;
-          holds_on_raw_data_item_eq (raw_data_item_sorted_elem order) (Map len v);
-          holds_on_raw_data_item_eq (raw_data_item_ints_optimal_elem) (Map len v);
-          assert (List.Tot.for_all (holds_on_pair (holds_on_raw_data_item raw_data_item_ints_optimal_elem)) v);
-          assert_norm (raw_data_item_ints_optimal == holds_on_raw_data_item raw_data_item_ints_optimal_elem);
-          assert (List.Tot.for_all (holds_on_pair raw_data_item_ints_optimal) v);
-          raw_data_item_sorted_optimal_valid_aux order v
-      | _ -> ()
-    )
-    x1
+
+let rec raw_equiv_list_no_map
+  (l1 l2: list raw_data_item)
+: Tot bool
+  (decreases (list_sum raw_data_item_size l1))
+= match l1, l2 with
+  | [], [] -> true
+  | x1 :: q1, x2 :: q2 ->
+    raw_data_item_size_eq x1;
+    begin match x1, x2 with
+    | Simple v1, Simple v2 -> v1 = v2 && raw_equiv_list_no_map q1 q2
+    | Int64 ty1 v1, Int64 ty2 v2 -> ty1 = ty2 && raw_uint64_equiv v1 v2 && raw_equiv_list_no_map q1 q2
+    | String ty1 len1 v1, String ty2 len2 v2 -> ty1 = ty2 && raw_uint64_equiv len1 len2 && v1 = v2 && raw_equiv_list_no_map q1 q2
+    | Array len1 v1, Array len2 v2 ->
+      list_sum_append raw_data_item_size v1 q1;
+      raw_uint64_equiv len1 len2 &&
+      raw_equiv_list_no_map (List.Tot.append v1 q1) (List.Tot.append v2 q2)
+    | Tagged tag1 v1, Tagged tag2 v2 ->
+      raw_uint64_equiv tag1 tag2 &&
+      raw_equiv_list_no_map (v1 :: q1) (v2 :: q2)
+    | _ -> false
+    end
+  | _ -> false
+
+val raw_equiv_list_no_map_append
+  (ll1 lr1 ll2 lr2: list raw_data_item)
+: Lemma
+  (requires (List.Tot.length ll1 == List.Tot.length ll2))
+  (ensures (raw_equiv_list_no_map (List.Tot.append ll1 lr1) (List.Tot.append ll2 lr2) == (raw_equiv_list_no_map ll1 ll2 && raw_equiv_list_no_map lr1 lr2)))
+
+val raw_equiv_list_no_map_no_map
+  (l1 l2: list raw_data_item)
+: Lemma
+  (requires (raw_equiv_list_no_map l1 l2 == true))
+  (ensures (List.Tot.for_all (holds_on_raw_data_item (notp Map?)) l1 == true))
+
+val raw_equiv_list_no_map_equiv
+  (l1 l2: list raw_data_item)
+: Lemma
+  (requires (raw_equiv_list_no_map l1 l2 == true))
+  (ensures (list_for_all2 raw_equiv l1 l2 == true))
+
+val raw_equiv_list_no_map_sym
+  (l1 l2: list raw_data_item)
+: Lemma
+  (raw_equiv_list_no_map l1 l2 == raw_equiv_list_no_map l2 l1)
+
+val raw_equiv_equiv_list_no_map
+  (l1 l2: list raw_data_item)
+: Lemma
+  (requires (
+    list_for_all2 raw_equiv l1 l2 == true /\
+    list_for_all2 (prod_or (holds_on_raw_data_item (notp Map?)) (holds_on_raw_data_item (notp Map?))) l1 l2 == true
+  ))
+  (ensures (
+    raw_equiv_list_no_map l1 l2 == true
+  ))
+
+val raw_equiv_list_no_map_eq
+  (l1 l2: list raw_data_item)
+: Lemma
+  (raw_equiv_list_no_map l1 l2 == (list_for_all2 raw_equiv l1 l2 && list_for_all2 (prod_or (holds_on_raw_data_item (notp Map?)) (holds_on_raw_data_item (notp Map?))) l1 l2))
+
+let raw_equiv_no_map
+  (x1 x2: raw_data_item)
+: Tot bool
+= raw_equiv_list_no_map [x1] [x2]
+
+let raw_equiv_list_no_map_no_map2
+  (l1 l2: list raw_data_item)
+: Lemma
+  (requires (raw_equiv_list_no_map l1 l2 == true))
+  (ensures (List.Tot.for_all (holds_on_raw_data_item (notp Map?)) l1 == true /\
+    List.Tot.for_all (holds_on_raw_data_item (notp Map?)) l2 == true
+  ))
+= raw_equiv_list_no_map_no_map l1 l2;
+  raw_equiv_list_no_map_sym l1 l2;
+  raw_equiv_list_no_map_no_map l2 l1
+
+val raw_equiv_list_no_map_eq'
+  (l1 l2: list raw_data_item)
+: Lemma
+  (ensures (raw_equiv_list_no_map l1 l2 == list_for_all2 raw_equiv_no_map l1 l2))
+
+let no_maps_in_keys_map
+  (v: list (raw_data_item & raw_data_item))
+: Tot bool
+= List.Tot.for_all (holds_on_raw_data_item (notp Map?)) (List.Tot.map fst v)
+
+let no_maps_in_keys_elem
+  (l: raw_data_item)
+: Tot bool
+= match l with
+  | Map _ v -> no_maps_in_keys_map v
+  | _ -> true
+
+let no_maps_in_keys = holds_on_raw_data_item no_maps_in_keys_elem
+
+
+let valid_raw_data_item_no_maps_in_keys_map
+  (v: list (raw_data_item & raw_data_item))
+: Tot bool
+= list_no_setoid_repeats (map_entry_order raw_equiv_no_map _) v
+
+let valid_raw_data_item_no_maps_in_keys_elem_gen
+  (p: raw_data_item -> bool)
+  (l: raw_data_item)
+: Tot bool
+= p l &&
+  begin match l with
+  | Map _ v -> valid_raw_data_item_no_maps_in_keys_map v
+  | _ -> true
+  end
+
+let valid_raw_data_item_no_maps_in_keys_elem =
+  valid_raw_data_item_no_maps_in_keys_elem_gen no_maps_in_keys_elem
+
+let valid_raw_data_item_no_maps_in_keys_gen
+  (p: raw_data_item -> bool)
+: Tot (raw_data_item -> bool)
+= holds_on_raw_data_item (valid_raw_data_item_no_maps_in_keys_elem_gen p)
+
+let valid_raw_data_item_no_maps_in_keys = holds_on_raw_data_item valid_raw_data_item_no_maps_in_keys_elem
+
+val valid_no_maps_in_keys_no_maps_in_keys_gen
+  (p: raw_data_item -> bool)
+  (x: raw_data_item)
+: Lemma
+  (requires (valid_raw_data_item_no_maps_in_keys_gen p x == true))
+  (ensures (holds_on_raw_data_item p x == true))
+
+let valid_no_maps_in_keys_no_maps_in_keys
+  (x: raw_data_item)
+: Lemma
+  (requires (valid_raw_data_item_no_maps_in_keys x == true))
+  (ensures (no_maps_in_keys x == true))
+= assert_norm (valid_raw_data_item_no_maps_in_keys == valid_raw_data_item_no_maps_in_keys_gen no_maps_in_keys_elem);
+  valid_no_maps_in_keys_no_maps_in_keys_gen no_maps_in_keys_elem x
+
+val valid_no_maps_in_keys_valid_map
+  (l: list (raw_data_item & raw_data_item))
+: Lemma
+  (requires (
+    List.Tot.for_all (holds_on_pair valid_raw_data_item_no_maps_in_keys) l == true /\
+    no_maps_in_keys_map l == true /\
+    valid_raw_data_item_no_maps_in_keys_map l == true
+  ))
+  (ensures (
+    valid_raw_data_item_map l == true
+  ))
+
+val valid_no_maps_in_keys_valid
+  (x: raw_data_item)
+: Lemma
+  (requires (valid_raw_data_item_no_maps_in_keys x == true))
+  (ensures (valid_raw_data_item x == true))
+
+val valid_no_maps_in_keys_valid_gen
+  (p: raw_data_item -> bool)
+  (x: raw_data_item)
+: Lemma
+  (requires (
+    valid_raw_data_item_no_maps_in_keys_gen p x == true /\
+    (forall x' . p x' == true ==> no_maps_in_keys_elem x' == true)
+  ))
+  (ensures (valid_raw_data_item x == true))
+
+val valid_valid_no_maps_in_keys_gen
+  (p: raw_data_item -> bool)
+  (x: raw_data_item)
+: Lemma
+  (requires (valid_raw_data_item x == true /\
+    holds_on_raw_data_item p x == true
+  ))
+  (ensures (valid_raw_data_item_no_maps_in_keys_gen p x == true))
+
+val valid_valid_no_maps_in_keys
+  (x: raw_data_item)
+: Lemma
+  (requires (valid_raw_data_item x == true /\
+    no_maps_in_keys x == true
+  ))
+  (ensures (valid_raw_data_item_no_maps_in_keys x == true))
+
+val valid_raw_data_item_no_maps_in_keys_eq
+  (x: raw_data_item)
+: Lemma
+  (valid_raw_data_item_no_maps_in_keys x ==
+    (valid_raw_data_item x && no_maps_in_keys x)
+  )
+
+val valid_raw_data_item_no_maps_in_keys_gen_eq
+  (p: raw_data_item -> bool)
+  (x: raw_data_item)
+: Lemma
+  (requires (
+    forall x' . p x' == true ==> no_maps_in_keys_elem x' == true
+  ))
+  (ensures (valid_raw_data_item_no_maps_in_keys_gen p x ==
+    (valid_raw_data_item x && holds_on_raw_data_item p x)
+  ))
+
